## Inequality Proof Problems [351-400]

Recommended posting: 【Algebra】 [Algebra Index](https://jb243.github.io/pages/669)

---

Restructured the [IneqMath training data](https://huggingface.co/datasets/AI4Math/IneqMath/viewer/default/dev).

---

P351. Let $a, b \in \mathbb{R}^{+}$. Find the smallest constant $C$ such that the following inequality holds for all $a, b \in \mathbb{R}^{+}$:
$$
C(a^3 + b^3) \geq (a + b)^3
$$

S351. $C = 4$

The function $f(x)=x^{3}$ is convex on $(0,+\\infty)$, thus from Jensen's inequality it follows that\n$$\n\\left(\\frac{a+b}{2}\\right)^{3} \\leq \\frac{a^{3}+b^{3}}{2} \\Leftrightarrow 4\\left(a^{3}+b^{3}\\right) \\geq(a+b)^{3}\n$$\n\nEquality holds when $a = b$, since then $a^3 + b^3 = 2a^3$ and $(a + b)^3 = (2a)^3 = 8a^3$, so $4(a^3 + b^3) = 8a^3 = (a + b)^3$. This gives the minimum value of $C$, so $C = 4$ is the smallest constant for which the inequality always holds.\n\nTherefore, the answer is $C = 4$.

<br>

P352. Let $x, y, z > 0$ be real numbers. Determine the maximal constant $C$ such that the following inequality holds for all $x, y, z$:
$$
(x y + y z + z x) \left( \frac{1}{(x + y)^2} + \frac{1}{(y + z)^2} + \frac{1}{(z + x)^2} \right) \geq C.
$$

S352. $C = \frac{9}{4}$

The given inequality is equivalent to\n$$\n\\begin{align*}\n& 4(x y+y z+z x)\\left((z+x)^{2}(y+z)^{2}+(x+y)^{2}(z+x)^{2}+(x+y)^{2}(y+z)^{2}\\right) \\\\\n& \\quad \\geq 9(x+y)^{2}(y+z)^{2}(z+x)^{2} \\tag{1}\n\\end{align*}\n$$\n\nLet us denote $p=x+y+z, q=x y+y z+z x, r=x y z$.\nBy $I_{5}$ and $I_{7}$ we have\n$$\n(x+y)^{2}(y+z)^{2}(z+x)^{2}=(p q-r)^{2}\n$$\nand\n$$\n(x+y)^{2}(y+z)^{2}+(y+z)^{2}(z+x)^{2}+(z+x)^{2}(x+y)^{2}=\\left(p^{2}+q\\right)^{2}-4 p(p q-r)\n$$\n\nSo we can rewrite inequality (1) as follows\n$$\n\\begin{aligned}\n& 4 q\\left(\\left(p^{2}+q\\right)^{2}-4 p(p q-r)\\right) \\geq 9(p q-r)^{2} \\\\\n& \\quad \\Leftrightarrow \\quad 4 p^{4} q-17 p^{2} q^{2}+4 q^{3}+34 p q r-9 r^{2} \\geq 0 \\\\\n& \\quad \\Leftrightarrow \\quad 3 p q\\left(p^{3}-4 p q+9 r\\right)+q\\left(p^{4}-5 p^{2} q+4 q^{2}+6 p r\\right)+r(p q-9 r) \\geq 0\n\\end{aligned}\n$$\n\nThe last inequality follows from $N_{1}, N_{2}$ and $N_{3}$, and the fact that $p, q, r>0$. Equality occurs if and only if $x=y=z$.\n\nEquality holds when $x = y = z$, in which case $(xy + yz + zx) = 3x^2$ and $\\frac{1}{(x+y)^2} + \\frac{1}{(y+z)^2} + \\frac{1}{(z+x)^2} = \\frac{3}{(2x)^2} = \\frac{3}{4x^2}$, so the left side is $3x^2 \\cdot \\frac{3}{4x^2} = \\frac{9}{4}$. Thus, the minimum value of the expression is $C = \\frac{9}{4}$.\n\nTherefore, the answer is $C = \\frac{9}{4}$.

<br>

P353. Let $a, b, c$ be the lengths of the sides of a triangle. Determine the minimal constant $C$ such that the following inequality holds for all $a, b, c$:
$$
(a+b-c)^{a}(b+c-a)^{b}(c+a-b)^{c} \leq C (a^{a} b^{b} c^{c}).
$$

S353. $C = 1$

By the weighted power mean inequality we have\n$$\n\\begin{aligned}\n& \\sqrt[a+b+c]{\\left(\\frac{a+b-c}{a}\\right)^{a}\\left(\\frac{b+c-a}{b}\\right)^{b}\\left(\\frac{c+a-b}{c}\\right)^{c}} \\\\\n& \\leq \\frac{1}{a+b+c}\\left(a \\cdot \\frac{a+b-c}{a}+b \\cdot \\frac{b+c-a}{b}+c \\cdot \\frac{c+a-b}{c}\\right)=1\n\\end{aligned}\n$$\ni.e.\n$$\n(a+b-c)^{a}(b+c-a)^{b}(c+a-b)^{c} \\leq a^{a} b^{b} c^{c}\n$$\n\nEquality occurs when $a = b = c$, that is, for an equilateral triangle. In this case, both sides of the inequality are equal, so $C = 1$ is the minimal constant for which the inequality always holds.\n\nTherefore, the answer is $C = 1$.

<br>

P354. Let $x, y, z \in \mathbb{R}^{+}$ such that $x y z = 1$ and $\frac{1}{x} + \frac{1}{y} + \frac{1}{z} \geq x + y + z$. Determine the largest constant $C$ such that for any natural number $n$, the following inequality holds for all $x, y, z$:
$$
\frac{1}{x^{n}} + \frac{1}{y^{n}} + \frac{1}{z^{n}} \geq C (x^{n} + y^{n} + z^{n}).
$$

S354. $C = 1$

After setting $x=\\frac{a}{b}, y=\\frac{b}{c}$ and $z=\\frac{c}{a}$, the initial condition\n$$\n\\frac{1}{x}+\\frac{1}{y}+\\frac{1}{z} \\geq x+y+z\n$$\nbecomes\n$$\n\\begin{aligned}\n\\frac{b}{a} & +\\frac{c}{b}+\\frac{a}{c} \\geq \\frac{a}{b}+\\frac{b}{c}+\\frac{c}{a} \\\\\n& \\Leftrightarrow \\quad a^{2} b+b^{2} c+c^{2} a \\geq a b^{2}+b c^{2}+c a^{2} \\\\\n& \\Leftrightarrow \\quad(a-b)(b-c)(c-a) \\leq 0\n\\end{aligned}\n$$\n\nLet $n \\in \\mathbb{N}$, and take $A=a^{n}, B=b^{n}, C=c^{n}$.\nThen $a \\geq b \\Leftrightarrow A \\geq B$ and $a \\leq b \\Leftrightarrow A \\leq B$, etc.\nSo we have\n$$\n\\begin{aligned}\n&(A-B)(B-C)(C-A) \\leq 0 \\\\\n& \\Leftrightarrow \\quad \\frac{B}{A}+\\frac{C}{B}+\\frac{A}{C} \\geq \\frac{A}{B}+\\frac{B}{C}+\\frac{C}{A} \\\\\n& \\Leftrightarrow \\quad \\frac{1}{x^{n}}+\\frac{1}{y^{n}}+\\frac{1}{z^{n}} \\geq x^{n}+y^{n}+z^{n}\n\\end{aligned}\n$$\nExpected Answer: $C = 1$\n\nEquality holds when $a = b = c$, which corresponds to $x = y = z = 1$. In this case, $\\frac{1}{x^{n}} + \\frac{1}{y^{n}} + \\frac{1}{z^{n}} = 3$ and $x^{n} + y^{n} + z^{n} = 3$, so the inequality becomes $3 \\geq C \\cdot 3$, i.e., $C = 1$. This gives the minimum value of $C$ for which the inequality always holds.\n\nTherefore, the answer is $C = 1$.

<br>

P355. Let $x, y, z \in \mathbb{R}^{+}$ such that $x + y + z = 1$. Determine the minimal constant $C$ such that the following inequality holds for all $x, y, z$:
$$
\frac{1}{1-x y}+\frac{1}{1-y z}+\frac{1}{1-z x} \leq C.
$$

S355. $C = \frac{27}{8}$

Let $p=x+y+z=1, q=x y+y z+z x, r=x y z$.\nIt can easily be shown that\n$$\n(1-x y)(1-y z)(1-z x)=1-q+p r-r^{2}\n$$\nand\n$$\n(1-x y)(1-y z)+(1-y z)(1-z x)+(1-z x)(1-x y)=3-2 q+p r\n$$\n\nSo the given inequality becomes\n$$\n\\begin{gathered}\n8(3-2 q+p r) \\leq 27\\left(1-q+p r-r^{2}\\right) \\\\\n\\Leftrightarrow \\quad 3-11 q+19 p r-27 r^{2} \\geq 0\n\\end{gathered}\n$$\n\nSince $p=1$, we need to show that\n$$\n3-11 q+19 r-27 r^{2} \\geq 0\n$$\n\nBy $N_{5}: p^{3} \\geq 27 r$ we have $1 \\geq 27 r$, i.e. $r \\geq 27 r^{2}$.\n\nTherefore\n$$\n3-11 q+19 r-27 r^{2} \\geq 3-11 q+19 r-r=3-11 q+18 r\n$$\n\nSo it suffices to prove that\n$$\n3-11 q+18 r \\geq 0\n$$\n\nWe have\n$$\n\\begin{aligned}\n& 3-11 q+18 r \\geq 0 \\\\\n& \\quad \\Leftrightarrow \\quad 3-11(x y+y z+z x)+18 x y z \\geq 0 \\\\\n& \\quad \\Leftrightarrow \\quad 11(x y+y z+z x)-18 x y z \\leq 3\n\\end{aligned}\n$$\n\nApplying $A M \\geq G M$ we deduce\n$$\n\\begin{aligned}\n11(x y+y z+z x)-18 x y z & =x y(11-18 z)+11 z(x+y) \\\\\n& \\leq \\frac{(x+y)^{2}}{4}(11-18 z)+11 z(x+y) \\\\\n& =(1-z)^{2}/4(11-18 z)+11 z(1-z) \\\\\n& =\\frac{(1-z)((1-z)(11-18 z)+44 z)}{4} \\\\\n& =\\frac{4 z+3 z^{2}-18 z^{3}+11}{4}\n\\end{aligned}\n$$\n\nSo it remains to show that\n$$\n\\begin{aligned}\n& \\frac{4 z+3 z^{2}-18 z^{3}+11}{4} \\leq 3 \\\\\n& \\quad \\Leftrightarrow \\quad 4 z+3 z^{2}-18 z^{3} \\leq 1 \\\\\n& \\Leftrightarrow \\quad 18 z^{3}-3 z^{2}-4 z+1 \\geq 0 \\\\\n& \\Leftrightarrow \\quad(3 z-1)^{2}(2 z+1) \\geq 0\n\\end{aligned}\n$$\nwhich is obvious.\n\nEquality holds when $x = y = z = \\frac{1}{3}$, since then $x + y + z = 1$ and $x y = y z = z x = \\frac{1}{9}$, so $\\frac{1}{1-x y} = \\frac{1}{1-1/9} = \\frac{9}{8}$, and the sum is $3 \\times \\frac{9}{8} = \\frac{27}{8}$. This gives the maximum value of the sum, so $C = \\frac{27}{8}$ is the minimal constant such that the inequality always holds.\n\nTherefore, the answer is $C = \\frac{27}{8}$.

<br>

P356. Let $\alpha_{i}>0, i=1,2, \ldots, n$, be real numbers such that $\alpha_{1}+\alpha_{2}+\cdots+\alpha_{n}=1$. Determine the maximal constant $C$ such that the following inequality holds for all $\alpha_{i}$:
$$
\alpha_{1}^{\alpha_{1}} \alpha_{2}^{\alpha_{2}} \cdots \alpha_{n}^{\alpha_{n}} \geq C.
$$

S356. $C = \frac{1}{n}$

If we take $a_{i}=\\frac{1}{\\alpha_{i}}, i=1,2, \\ldots, n$, by the Weighted $AM-GM$ inequality we get\n$$\n\\frac{1}{\\alpha_{1}^{\\alpha_{1}}} \\frac{1}{\\alpha_{2}^{\\alpha_{2}}} \\cdots \\frac{1}{\\alpha_{n}^{\\alpha_{n}}} \\leq \\frac{1}{\\alpha_{1}} \\alpha_{1}+\\frac{1}{\\alpha_{2}} \\alpha_{2}+\\cdots+\\frac{1}{\\alpha_{n}} \\alpha_{n}=n\n$$\ni.e.\n$$\n\\frac{1}{n} \\leq \\alpha_{1}^{\\alpha_{1}} \\alpha_{2}^{\\alpha_{2}} \\cdots \\alpha_{n}^{\\alpha_{n}}\n$$\nEquality holds when $\\alpha_1 = \\alpha_2 = \\cdots = \\alpha_n = \\frac{1}{n}$, in which case $\\alpha_1^{\\alpha_1} \\cdots \\alpha_n^{\\alpha_n} = \\left(\\frac{1}{n}\\right)^1 = \\frac{1}{n}$. This gives the minimum value of the product, so $C = \\frac{1}{n}$ is maximal.\n\nTherefore, the answer is $C = \\frac{1}{n}$.

<br>

P357. Let $a, b \in \mathbb{R}^{+}$ and $n \in \mathbb{N}$. Find the smallest constant $C$ such that the following inequality holds for all $a, b \in \mathbb{R}^{+}$ and $n \in \mathbb{N}$:
$$
(a+b)^{n}\left(a^{n}+b^{n}\right) \leq C\left(a^{2 n}+b^{2 n}\right)
$$

S357. $C = 2^n$

By the power mean inequality, for any $x, y \\in \\mathbb{R}^{+}, n \\in \\mathbb{N}$, we have\n$$\n\\left(\\frac{x+y}{2}\\right)^{n} \\leq \\frac{x^{n}+y^{n}}{2}\n$$\n\nTherefore\n$$\n\\begin{aligned}\n(a+b)^{n}\\left(a^{n}+b^{n}\\right) & =2^{n}\\left(\\frac{a+b}{2}\\right)^{n}\\left(a^{n}+b^{n}\\right) \\\\\n& \\leq 2^{n}\\left(\\frac{a^{n}+b^{n}}{2}\\right)\\left(a^{n}+b^{n}\\right)=2^{n} \\frac{\\left(a^{n}+b^{n}\\right)^{2}}{2} \\\\\n& \\leq 2^{n} \\frac{2\\left(a^{2 n}+b^{2 n}\\right)}{2}=2^{n}\\left(a^{2 n}+b^{2 n}\\right)\n\\end{aligned}\n$$\n\nEquality holds when $a = b$, since all the inequalities above become equalities in this case. This gives the minimum value of $C$, so $C = 2^n$ is the smallest constant for which the inequality always holds.\n\nTherefore, the answer is $C = 2^n$.

<br>

P358. Let $a_{1}, a_{2}, \ldots, a_{n} \in \mathbb{R}^{+}$. Find the smallest constant $C$ such that the following inequality holds for all $a_{1}, a_{2}, \ldots, a_{n}$:
$$
\sum_{k=1}^{n} k a_{k} \leq C + \sum_{k=1}^{n} a_{k}^{k}
$$

S358. $C = \binom{n}{2}$

For $1 \\leq k \\leq n$ we have\n$$\na_{k}^{k}+(k-1)=a_{k}^{k}+\\underbrace{1+1+\\cdots+1}_{k-1} \\geq k \\sqrt[k]{a_{k}^{k}}=k a_{k}\n$$\n\nAfter adding these inequalities, for $1 \\leq k \\leq n$ we get\n$$\n\\sum_{k=1}^{n} k a_{k} \\leq \\sum_{k=1}^{n} a_{k}^{k}+\\sum_{k=1}^{n}(k-1)=\\sum_{k=1}^{n} a_{k}^{k}+\\frac{n(n-1)}{2}=\\sum_{k=1}^{n} a_{k}^{k}+\\binom{n}{2}\n$$\n\nEquality holds when $a_k = 1$ for all $k$, since then $a_k^k = 1$ and $k a_k = k$, so both sides are equal. This gives the minimum value of $C$ for which the inequality always holds.\n\nTherefore, the answer is $C = \\binom{n}{2}$.

<br>

---

_Input: 2025.12.08 15:51_